misc/miscScript.sml
@@ -3,7 +3,7 @@
    development.
 *)
 
-open HolKernel bossLib boolLib boolSimps Parse libTheory mp_then
+open HolKernel bossLib boolLib boolSimps Parse mp_then
 open alignmentTheory alistTheory arithmeticTheory bitstringTheory bagTheory
      byteTheory combinTheory dep_rewrite containerTheory listTheory
      pred_setTheory finite_mapTheory rich_listTheory llistTheory optionTheory
@@ -15,6 +15,19 @@ local open bagLib addressTheory blastLib in end
 (* Misc. lemmas (without any compiler constants) *)
 val _ = new_theory "misc"
 val _ = ParseExtras.tight_equality()
+
+(* Total version of THE *)
+Definition the_def:
+  the _ (SOME x) = x ∧
+  the x NONE =  x
+End
+
+Definition opt_bind_def:
+ opt_bind n v e =
+   case n of
+   | NONE => e
+   | SOME n' => (n',v)::e
+End
 
 (* Note: This globally hides constants over the reals that gets imported through machine_ieeeTheory *)
 
