candle/overloading/ml_checker/ml_cyclicityCheckerProgScript.sml
@@ -2,7 +2,7 @@
   An I/O shim for the verified cyclicity checker
 *)
 open preamble ml_translatorTheory ml_translatorLib ml_pmatchTheory patternMatchesTheory
-open astTheory libTheory evaluateTheory semanticPrimitivesTheory
+open astTheory evaluateTheory semanticPrimitivesTheory
 open ml_progLib ml_progTheory evaluateTheory
 open set_sepTheory cfTheory cfStoreTheory cfTacticsLib Satisfy
 open cfHeapsBaseTheory basisFunctionsLib
